Prove trivial_deterministic via AdvanceTage.RTC

src/ReactorModel/Determinism/Execution.lean
@@ -4,21 +4,32 @@ open Classical
 
 namespace Execution
 
-theorem trivial_rtr_eq [State.Trivial s₁] : (s₁ ⇓* s₂) → s₁.rtr = s₂.rtr
-  | refl      => rfl
-  | step e e' => 
-    have := e.preserves_Trivial -- TODO: Make this work via type class inference.
-    e.trivial_rtr_eq ▸ e'.trivial_rtr_eq
+-- This is only used for the proof of `trivial_deterministic`.
+inductive AdvanceTag.RTC : State → State → Type
+  | refl : RTC s s
+  | trans : (s₁ ⇓- s₂) → (RTC s₂ s₃) → RTC s₁ s₃   
 
-theorem trivial_ctx_eq [State.Trivial s₁] : (s₁ ⇓* s₂) →
-  s₂.ctx = (s₁.ctx.mark $ s₁.rtr.scheduledTags.filter fun g => s₁.tag < g ∧ g ≤ s₂.tag) :=
-    sorry
+-- This is only used for the proof of `trivial_deterministic`.
+theorem AdvanceTag.RTC.deterministic 
+  (a₁ : AdvanceTag.RTC s s₁) (a₂ : AdvanceTag.RTC s s₂) (ht : s₁.tag = s₂.tag) : s₁ = s₂ := by
+  induction a₁ <;> cases a₂
+  case refl.refl                       => rfl
+  case' refl.trans a _, trans.refl _ a => exact absurd ht a.tag_ne
+  case trans.trans a₁ _ hi _ a₂ c₂     => exact hi (a₂.determinisic a₁ ▸ c₂) ht
+
+-- This is only used for the proof of `trivial_deterministic`.
+def trivial_erase_exec_steps [State.Trivial s₁] : (s₁ ⇓* s₂) → AdvanceTag.RTC s₁ s₂
+  | refl => .refl
+  | step (.advance a) e' => 
+    have := a.preserves_Trivial -- TODO: Make this work via type class inference.
+    .trans a e'.trivial_erase_exec_steps
+  | step (.close e) e' => 
+    have := e.preserves_Trivial -- TODO: Make this work via type class inference.
+    e.trivial_eq ▸ e'.trivial_erase_exec_steps
 
 theorem trivial_deterministic [trivial : State.Trivial s] 
-    (e₁ : s ⇓* s₁) (e₂ : s ⇓* s₂) (ht : s₁.tag = s₂.tag) : s₁ = s₂ := by
-  ext1
-  · exact e₁.trivial_rtr_eq ▸ e₂.trivial_rtr_eq 
-  · rw [e₁.trivial_ctx_eq, e₂.trivial_ctx_eq, ht]
+    (e₁ : s ⇓* s₁) (e₂ : s ⇓* s₂) (ht : s₁.tag = s₂.tag) : s₁ = s₂ :=
+  AdvanceTag.RTC.deterministic e₁.trivial_erase_exec_steps e₂.trivial_erase_exec_steps ht
 
 theorem tag_le : (s₁ ⇓* s₂) → s₁.tag ≤ s₂.tag
   | refl      => le_refl _
@@ -45,6 +56,6 @@ theorem deterministic :
     (s ⇓* s₁) → (s ⇓* s₂) → (s₁.tag = s₂.tag) → (s₁.progress = s₂.progress) → s₁ = s₂ := 
   if h : State.Nontrivial s 
   then nontrivial_deterministic
-  else fun e₁ e₂ ht _ => trivial_deterministic e₁ e₂ ht (trivial := ⟨h⟩)
+  else fun e₁ e₂ ht _ => trivial_deterministic e₁ e₂ ht (trivial := .of_not_Nontrivial h)
   
 end Execution
